Progress on Analysis verification

Analysis.v
@@ -1,55 +1,55 @@
-Require Import CSet Le ListUpdateAt.
+Require Import CSet Le ListUpdateAt Coq.Classes.RelationClasses.
 
 Require Import Plus Util AllInRel Map Terminating.
-Require Import Val Var Env EnvTy IL Annotation Lattice DecSolve LengthEq MoreList Status AllInRel.
+Require Import Val Var Env EnvTy IL Annotation Lattice DecSolve LengthEq MoreList Status AllInRel OptionR.
 
 Set Implicit Arguments.
 
 (** Specification of an analysis and generic fixpoint iteration algorithm *)
 
-Class Analysis (Dom: Type) := makeAnalysis {
-  dom_po :> PartialOrder Dom;
-  analysis_step : stmt -> Dom -> Dom;
-  initial_value : stmt -> Dom;
-  finite_height : Terminating poLt;
-  step_monotone : forall s d, poLe d (analysis_step s d);
-  step_respectful :> Proper (eq ==> poEq ==> poEq) analysis_step
+Class Monotone Dom `{PartialOrder Dom} Dom' `{PartialOrder Dom'} (f:Dom->Dom') :=
+  monotone : forall a b, poLe a b -> poLe (f a) (f b).
+
+Class Analysis (Dom: stmt -> Type) := makeAnalysis {
+  dom_po :> forall sT, PartialOrder (Dom sT);
+  analysis_step : forall sT, stmt -> Dom sT -> Dom sT;
+  initial_value : forall sT, Dom sT;
+  initial_value_bottom : forall s d, poLe (initial_value s) d;
+  finite_height : forall (sT:stmt), Terminating (Dom sT) poLt;
+  step_monotone : forall sT s, Monotone (@analysis_step sT s)
 }.
 
+Hint Extern 5 =>
+match goal with
+  [ H : poLe ?d ?d' |- poLe (analysis_step _ ?s ?d) (analysis_step _ ?s ?d')] =>
+  eapply (step_monotone _ s _ _ H)
+end.
+
 Section AnalysisAlgorithm.
-  Variable Dom : Type.
+  Variable Dom : stmt -> Type.
   Variable analysis : Analysis Dom.
 
-  Fixpoint safeFirst (s:stmt) (d:Dom) (trm:terminates poLt d) : Dom.
-    refine (let d' := analysis_step s d in
-            if [poLe d' d] then d' else safeFirst s d' _).
-    destruct trm. eapply H.
-    eapply poLe_poLt; eauto.
-    eapply step_monotone.
+  Fixpoint safeFirst (sT s:stmt) (d:Dom sT) (mon:poLe d (analysis_step sT s d)) (trm:terminates poLt d)
+    : { d' : Dom sT | exists n : nat, d' = iter n d (fun _ => analysis_step sT s) /\ poEq (analysis_step sT s d') d' }.
+    decide (poLe (analysis_step sT s d) d).
+    - eexists (analysis_step sT s d), 1; simpl.
+      split; eauto.
+      eapply poLe_antisymmetric; eauto.
+    - destruct (safeFirst sT s (analysis_step sT s d)) as [d' H]; [ eauto | |].
+      + destruct trm. eapply H.
+        eapply poLe_poLt; eauto.
+      + eexists d'. destruct H as [n' H]. eexists (S n'); simpl. eauto.
   Defined.
 
-  Definition safeFixpoint (s:stmt) :=
-    @safeFirst s (initial_value s) (finite_height _).
-
-  Fixpoint safeFixpoint_iter s d d' trm
-    : @safeFirst s d trm = d'
-      -> exists n, d' = iter n d (fun _ => analysis_step s)
-        /\ poEq (analysis_step s d') d'.
-  Proof.
-    intros. destruct trm. simpl in *.
-    destruct (decision_procedure (poLe (analysis_step s x) x)).
-    + eexists 1; simpl. split; eauto.
-      assert (poEq x d').
-      pose proof (step_monotone s x).
-      rewrite H in p,H0.
-      eapply poLe_antisymmetric; eauto.
-      rewrite <- H0 at 1. rewrite H. reflexivity.
-    + destruct (safeFixpoint_iter _ _ _ _ H) as [n' ?].
-      eexists (S n'); eauto.
-  Qed.
+  Definition safeFixpoint (s:stmt)
+    : { d' : Dom s | exists n : nat, d' = iter n (initial_value s) (fun _ => analysis_step s s)
+                            /\ poEq (analysis_step s s d') d' }.
+    eapply @safeFirst.
+    - eapply initial_value_bottom.
+    - eapply finite_height.
+  Defined.
 
 End AnalysisAlgorithm.
-
 
 
 Inductive anni (A:Type) : Type :=
@@ -58,7 +58,6 @@ Inductive anni (A:Type) : Type :=
 | anni2 (a1:A) (a2:A) : anni A
 | anni2opt (a1:option A) (a2:option A) : anni A.
 
-Arguments anni A.
 Arguments anni0 [A].
 
 
@@ -69,54 +68,163 @@ Fixpoint setAnni {A} (a:ann A) (ai:anni A) : ann A :=
     | an, _ => an
   end.
 
-Inductive option_P {A} (P: A -> Prop) : option A -> Prop :=
-| option_P_None : option_P P (None)
-| option_R_Some a : P a -> option_P P (Some a).
+Inductive anni_R A B (R : A -> B -> Prop) : anni A -> anni B -> Prop :=
+| anni_R0
+  : anni_R R anni0 anni0
+| anni_R1 a1 a2
+  : R a1 a2 -> anni_R R (anni1 a1) (anni1 a2)
+| anni_R2 a1 a1' a2 a2'
+  : R a1 a2 -> R a1' a2' -> anni_R R (anni2 a1 a1') (anni2 a2 a2')
+| anni_R2o o1 o1' o2 o2'
+  : option_R R o1 o2 -> option_R R o1' o2' -> anni_R R (anni2opt o1 o1') (anni2opt o2 o2').
 
-Inductive anni_P {A} (P : A -> Prop) : anni A -> Prop :=
-| anni_P0 : anni_P P anni0
-| anni_P1 a : P a -> anni_P P (anni1 a)
-| anni_P2 a a' : P a -> P a' -> anni_P P (anni2 a a')
-| anni_P2o o o' : option_P P o -> option_P P o' -> anni_P P (anni2opt o o').
+Instance anni_R_refl {A} {R} `{Reflexive A R} : Reflexive (anni_R R).
+Proof.
+  hnf; intros; destruct x; eauto using anni_R, option_R.
+  econstructor; reflexivity.
+Qed.
 
-Definition backward Dom FunDom
-           (btransform : list FunDom -> stmt -> anni Dom -> Dom)
-           (bmkFunDom : params -> ann Dom -> FunDom) :=
+Instance anni_R_sym {A} {R} `{Symmetric A R} : Symmetric (anni_R R).
+Proof.
+  hnf; intros. inv H0; eauto using anni_R.
+  econstructor; symmetry; eauto.
+Qed.
+
+Instance anni_R_trans A R `{Transitive A R} : Transitive (anni_R R).
+Proof.
+  hnf; intros ? ? ? B C.
+  inv B; inv C; econstructor; eauto.
+  - etransitivity; eauto.
+  - etransitivity; eauto.
+Qed.
+
+Instance anni_R_equivalence A R `{Equivalence A R} : Equivalence (anni_R R).
+Proof.
+  econstructor; eauto with typeclass_instances.
+Qed.
+
+Instance anni_R_anti A R Eq `{EqA:Equivalence _ Eq} `{@Antisymmetric A Eq EqA R}
+  : @Antisymmetric _ (anni_R Eq) _ (anni_R R).
+Proof.
+  intros ? ? B C. inv B; inv C; eauto using anni_R.
+  econstructor; eapply option_R_anti; eauto.
+Qed.
+
+Instance anni_R_dec A B (R:A->B->Prop)
+         `{forall a b, Computable (R a b)} (a:anni A) (b:anni B) :
+  Computable (anni_R R a b).
+Proof.
+  destruct a,b; try dec_solve.
+  - decide (R a1 a0); dec_solve.
+  - decide (R a1 a0); decide (R a2 a3); dec_solve.
+  - decide (option_R R a1 a0); decide (option_R R a2 a3); dec_solve.
+Defined.
+
+Instance PartialOrder_ann Dom `{PartialOrder Dom}
+: PartialOrder (anni Dom) := {
+  poLe := anni_R poLe;
+  poLe_dec := @anni_R_dec _ _ poLe poLe_dec;
+  poEq := anni_R poEq;
+  poEq_dec := @anni_R_dec _ _ poEq poEq_dec;
+}.
+Proof.
+  - intros. inv H0; eauto 20 using @anni_R, poLe_refl.
+    econstructor; eapply (@poLe_refl _ (PartialOrder_option Dom)); eauto.
+Defined.
+
+Inductive option_Rs A B (R: A -> B -> Prop) : option A -> B -> Prop :=
+| option_R_None b : option_Rs R None b
+| option_R_Some a b : R a b -> option_Rs R (Some a) b.
+
+
+Instance PartialOrder_anni Dom `{PartialOrder Dom}
+: PartialOrder (anni Dom) := {
+  poLe := anni_R poLe;
+  poLe_dec := @anni_R_dec _ _ poLe poLe_dec;
+  poEq := anni_R poEq;
+  poEq_dec := @anni_R_dec _ _ poEq poEq_dec;
+}.
+Proof.
+  - intros. inv H0; eauto 20 using @anni_R, poLe_refl.
+    econstructor; eapply (@poLe_refl _ (PartialOrder_option Dom)); eauto.
+Defined.
+
+Instance option_Rs_dec A B (R:A->B->Prop)
+         `{forall a b, Computable (R a b)} (a:option A) (b:B) :
+  Computable (option_Rs R a b).
+Proof.
+  destruct a; try dec_solve.
+  decide (R a b); dec_solve.
+Defined.
+
+Inductive anni_Rs A B (R : A -> B -> Prop) : anni A -> B -> Prop :=
+| anni_Rs0 b
+  : anni_Rs R anni0 b
+| anni_Rs1 a1 b
+  : R a1 b -> anni_Rs R (anni1 a1) b
+| anni_Rs2 a1 a2 b
+  : R a1 b -> R a2 b -> anni_Rs R (anni2 a1 a2) b
+| anni_Rs2o o1 o2 b
+  : option_Rs R o1 b -> option_Rs R o2 b -> anni_Rs R (anni2opt o1 o2) b.
+
+Instance anni_Rs_dec A B (R:A->B->Prop)
+         `{forall a b, Computable (R a b)} (a:anni A) (b:B) :
+  Computable (anni_Rs R a b).
+Proof.
+  destruct a; try dec_solve.
+  - decide (R a1 b); dec_solve.
+  - decide (R a1 b); decide (R a2 b); dec_solve.
+  - decide (option_Rs R a1 b); decide (option_Rs R a2 b); dec_solve.
+Defined.
+
+Require Import Keep.
+
+Definition ifb (b b':bool) := if b then b' else false.
+
+Definition backward Dom
+           (btransform : list params -> list (option Dom) -> stmt -> anni (option Dom) -> option Dom) :=
   fix backward
-         (AL:list FunDom) (st:stmt) (a:ann Dom) {struct st} : ann Dom :=
+      (ZL:list (params)) (AL:list (option Dom)) (st:stmt) (a:ann (option Dom)) {struct st}
+  : ann (option Dom) * list bool :=
   match st, a with
     | stmtLet x e s as st, ann1 d ans =>
-      let ans' := backward AL s ans in
-      let ai := anni1 (getAnn ans') in
-      let d := (btransform AL st ai) in
-      ann1 d ans'
+      let ans' := backward ZL AL s ans in
+      let ai := anni1 (getAnn (fst ans')) in
+      let d := (btransform ZL AL st ai) in
+      (ann1 d (fst ans'), snd ans')
+
     | stmtIf x s t as st, ann2 d ans ant =>
-      let ans' := backward AL s ans in
-      let ant' := backward AL t ant in
-      let ai := anni2 (getAnn ans') (getAnn ant') in
-      let d' := (btransform AL st ai) in
-      ann2 d' ans' ant'
+      let ans' := backward ZL AL s ans in
+      let ant' := backward ZL AL t ant in
+      let ai := anni2 (getAnn (fst ans')) (getAnn (fst ant')) in
+      let d' := (btransform ZL AL st ai) in
+      (ann2 d' (fst ans') (fst ant'), zip orb (snd ans') (snd ant'))
 
     | stmtApp f Y as st, ann0 d as an =>
-      ann0 (btransform AL st anni0)
+      (ann0 (btransform ZL AL st anni0),
+       list_update_at (List.map (fun _ => false) AL) (counted f) true)
 
     | stmtReturn x as st, ann0 d as an =>
-      ann0 (btransform AL st anni0)
+      (ann0 (btransform ZL AL st anni0), List.map (fun _ => false) AL)
 
     | stmtExtern x f Y s as st, ann1 d ans =>
-      let ans' := backward AL s ans in
-      let ai := anni1 (getAnn ans') in
-      let d' := (btransform AL st ai) in
-      ann1 d' ans'
-    | stmtFun F t as st, annF d ans ant =>
-      let ans' := zip (fun Zs =>
-        backward (zip (fun Zs ans => bmkFunDom (fst Zs) ans) F ans ++ AL) (snd Zs)) F ans in
-      let AL' := zip (fun Zs ans => bmkFunDom (fst Zs) ans) F ans' ++ AL in
-      let ant' := backward AL' t ant in
-      let ai := anni1 (getAnn ant') in
-      let d' := btransform AL' st ai in
-      annF d' ans' ant'
-    | _, an => an
+      let ans' := backward ZL AL s ans in
+      let ai := anni1 (getAnn (fst ans')) in
+      let d' := (btransform ZL AL st ai) in
+      (ann1 d' (fst ans'), snd ans')
+
+    | stmtFun F t as st, annF d anF ant =>
+      let ALinit := getAnn ⊝ anF ++ AL in
+      let ZL' := List.map fst F ++ ZL in
+      let anF' := zip (fun Zs => backward ZL' ALinit (snd Zs)) F anF in
+      let AL' := getAnn ⊝ (fst ⊝ anF') ++ AL in
+      let ant' := backward ZL' AL' t ant in
+      let ai := anni1 (getAnn (fst ant')) in
+      let d' := btransform ZL' AL' st ai in
+      let cll := fold_left (fun ant ans => zip ifb ant ans) (snd ⊝ anF') (snd ant') in
+      (annF d' (zip (fun (b:bool) a => if b then a else setTopAnn a None ) cll (fst ⊝ anF')) (fst ant'),
+       cll)
+    | _, an => (an, List.map (fun x => false) AL)
   end.
 
 
@@ -137,33 +245,218 @@ Proof.
   inv H0; simpl; eauto.
 Qed.
 
-Lemma backward_increasing Dom FunDom `{PartialOrder Dom}
-      (f : list FunDom -> stmt -> anni Dom -> Dom)
-      (fOK:forall AL s ai, anni_P (fun x => poLe x (f AL s ai)) ai)
-           (bmkFunDom : params -> ann Dom -> FunDom)
-  : forall AL (s : stmt) (d : ann Dom), d ⊑ backward f bmkFunDom AL s d.
+Definition impb (a b:bool) : Prop := if a then b else True.
+
+Instance PartialOrder_bool
+: PartialOrder bool := {
+  poLe := impb;
+  poLe_dec := _;
+  poEq := eq;
+  poEq_dec := _;
+}.
 Proof.
-  intros.
-  general induction s; destruct d; simpl; try reflexivity.
-  - econstructor.
-    btransform f fOK.
-    rewrite <- IHs; eauto.
+  - intros. unfold impb. hnf. destruct d, d'; try dec_solve; eauto.
+  - hnf; unfold impb. intros. destruct d,d'; simpl; eauto using bool.
+    congruence.
+  - hnf; unfold impb. intros. destruct x,y,z; simpl; eauto.
+  - hnf; unfold impb. intros. destruct x,y; eauto. exfalso; eauto.
+Defined.
 
-    eapply IHs; eauto.
-
+Instance implbb_refl : Reflexive impb.
+Proof.
+  hnf; destruct x; simpl; eauto.
 Qed.
 
-Instance makeBackwardAnalysis Dom FunDom (BSL:BoundedSemiLattice Dom)
-           (btransform : list FunDom -> stmt -> anni Dom -> Dom)
-           (bmkFunDom : params -> ann Dom -> FunDom) (trm:Terminating poLt)
-  : Analysis (ann Dom) := {
-                           analysis_step s d := backward btransform bmkFunDom nil s d;
-                           initial_value s := setAnn bottom s
-                         }.
+Lemma tab_false_impb Dom `{PartialOrder Dom} AL AL'
+  : poLe AL AL'
+    -> PIR2 impb (tab false ‖AL‖) (tab false ‖AL'‖).
 Proof.
-  eapply terminating_ann; eauto.
+  intros. hnf in H0.
+  general induction H0; simpl; unfold impb; eauto using @PIR2.
+Qed.
+
+Lemma zip_orb_impb Dom `{PartialOrder Dom} AL AL' BL BL'
+  : poLe AL AL'
+    -> poLe BL BL'
+    -> PIR2 impb (orb ⊜ AL BL) (orb ⊜ AL' BL').
+Proof.
+  unfold poLe; simpl.
+  intros A B.
+  general induction A; inv B; simpl; eauto using PIR2.
+  - econstructor; eauto.
+    unfold impb. destruct x, x0, y, y0; simpl in *; eauto.
+Qed.
+
+Hint Extern 5 (Is_true true) => eapply I.
+
+Lemma update_at_impb Dom `{PartialOrder Dom} AL AL' n
+  : poLe AL AL'
+    ->  PIR2 impb (list_update_at (tab false ‖AL‖) n true)
+            (list_update_at (tab false ‖AL'‖) n true).
+Proof.
+  unfold poLe; simpl.
+  intros A. general induction A; simpl; eauto using PIR2.
+  - unfold impb. destruct n; simpl; eauto using @PIR2, tab_false_impb.
+Qed.
+
+Lemma backward_monotone Dom `{PartialOrder Dom}
+      (f : list params -> list (option Dom) -> stmt -> anni (option Dom) -> option Dom)
+      (fMon:forall s ZL AL AL', poLe AL AL' ->
+                           forall a b, a ⊑ b -> f ZL AL s a ⊑ f ZL AL' s b)
+  : forall (s : stmt) ZL AL AL',
+    poLe AL AL' ->
+    forall a b : ann (؟ Dom), a ⊑ b -> backward f ZL AL s a ⊑ backward f ZL AL' s b.
+Proof.
+  intros s.
+  sind s; destruct s; intros ZL AL AL' ALLE d d' LE; simpl; inv LE; simpl;
+    eauto 10 using @ann_R, tab_false_impb, update_at_impb, zip_orb_impb.
+  - split; eauto. econstructor; eauto.
+    + eapply fMon; eauto.
+      econstructor.
+      eapply getAnn_poLe. eapply (IH s); eauto.
+    + eapply IH; eauto.
+    + eapply IH; eauto.
+  - split. econstructor; eauto.
+    + eapply fMon; eauto.
+      econstructor; eapply getAnn_poLe.
+      eapply (IH s1); eauto.
+      eapply (IH s2); eauto.
+    + eapply IH; eauto.
+    + eapply IH; eauto.
+    + eapply zip_orb_impb; eauto.
+      eapply IH; eauto.
+      eapply IH; eauto.
+  - split. econstructor; eauto.
+    + eapply fMon; eauto.
+    + eapply update_at_impb; eauto.
+  - split; eauto using tab_false_impb.
+    + econstructor; eapply fMon; eauto.
+  - split; eauto. econstructor; eauto.
+    + eapply fMon; eauto.
+      econstructor.
+      eapply getAnn_poLe. eapply (IH s); eauto.
+    + eapply IH; eauto.
+    + eapply IH; eauto.
+  - assert ( getAnn
+               ⊝ fst
+               ⊝ (fun Zs : params * stmt => backward f (fst ⊝ s ++ ZL) (getAnn ⊝ ans ++ AL) (snd Zs)) ⊜ s ans ++ AL
+               ⊑ getAnn
+               ⊝ fst
+               ⊝ (fun Zs : params * stmt => backward f (fst ⊝ s ++ ZL) (getAnn ⊝ bns ++ AL') (snd Zs)) ⊜ s
+               bns ++ AL'). {
+      eapply PIR2_app; eauto.
+      eapply PIR2_get; intros; inv_get.
+      eapply getAnn_poLe. eapply IH; eauto.
+      eapply PIR2_app; eauto.
+      eapply PIR2_get; intros; inv_get; try eapply getAnn_poLe; eauto with len.
+      exploit H2; eauto. eapply H2; eauto.
+      repeat rewrite map_length.
+      repeat rewrite zip_length2; eauto.
+      admit. admit.
+    }
+    simpl; split.
+    + econstructor; eauto.
+      * eapply fMon; eauto.
+        econstructor.
+        eapply getAnn_poLe. eapply IH; eauto.
+      * repeat rewrite zip_length2; eauto. admit.
+        admit. admit.
+      * intros; inv_get. admit.
+      * eapply IH; eauto.
+    + admit.
+Admitted.
+
+Lemma backward_annotation Dom `{PartialOrder Dom} s
+      (f : list params -> list (option Dom) -> stmt -> anni (option Dom) -> option Dom)
+  : forall ZL AL sT a, annotation sT a
+                  -> annotation sT (fst (backward f ZL AL s a)).
+Proof.
+  sind s; intros ZL AL sT a Ann; destruct s; inv Ann; simpl; eauto using @annotation.
+  - econstructor; eauto.
+    + rewrite zip_length2; eauto.
+      admit. admit.
+    + intros. inv_get.
+      destruct x.
+      * eapply IH; eauto.
+      * eapply setTopAnn_annotation.
+        eapply IH; eauto.
+Admitted.
 
 
+
+Instance PartialOrder_sig Dom `{PartialOrder Dom} (P:Dom -> Prop)
+: PartialOrder { x :Dom | P x } := {
+  poLe x y := poLe (proj1_sig x) (proj1_sig y);
+  poLe_dec := _;
+  poEq x y := poEq (proj1_sig x) (proj1_sig y);
+  poEq_dec := _;
+}.
+Proof.
+  - econstructor; hnf; intros; destruct x; try destruct y; try destruct z; simpl in *.
+    + reflexivity.
+    + symmetry; eauto.
+    + etransitivity; eauto.
+  - intros [a b] [c d]; simpl. eapply poLe_refl.
+  - intros [a b] [c d] [e f]; simpl; intros.
+    etransitivity; eauto.
+  - intros [a b] [c d]; simpl; intros.
+    eapply poLe_antisymmetric; eauto.
+Defined.
+
+
+Lemma terminating_sig Dom `{PO:PartialOrder Dom}
+  : Terminating Dom poLt
+    -> forall P, Terminating { x : Dom | P x } poLt.
+Proof.
+  intros Trm P [x Px].
+  specialize (Trm x).
+  induction Trm.
+  econstructor.
+  intros [y Py] [LE NEQ]; simpl in *.
+  eapply H0. split; eauto.
+Qed.
+
+
+Lemma ann_bottom s' (Dom:Type) `{BoundedSemiLattice Dom}
+  :  forall (d : ann Dom), annotation s' d -> setAnn bottom s' ⊑ d.
+Proof.
+  sind s'; destruct s'; simpl; intros d' Ann; inv Ann; simpl; eauto using @ann_R, bottom_least.
+  - econstructor; eauto using bottom_least.
+    eapply (IH s'); eauto.
+  - econstructor; eauto using bottom_least.
+    eapply IH; eauto.
+    eapply IH; eauto.
+  - econstructor. eauto using bottom_least.
+    eapply IH; eauto.
+  - econstructor; eauto using bottom_least with len.
+    + intros; inv_get. eapply IH; eauto.
+    + eapply IH; eauto.
+Qed.
+
+
+Instance makeBackwardAnalysis (Dom:stmt -> Type)
+         `{forall s, PartialOrder (Dom s)} (BSL:forall s, BoundedSemiLattice (option (Dom s)))
+         (f :forall s, list params -> list (option (Dom s)) -> stmt -> anni (option (Dom s)) -> option (Dom s))
+         (fMon:forall (s s':stmt) ZL AL AL', poLe AL AL' ->
+                                        forall a b, a ⊑ b -> f s ZL AL s' a ⊑ f s ZL AL' s' b)
+         (Trm: forall s, Terminating (Dom s) poLt)
+  : Analysis (fun s => { a : ann (option (Dom s)) | annotation s a }) :=
+             {
+               initial_value :=  fun s : stmt =>
+                  exist (fun a : ann (؟ (Dom s)) => annotation s a) (setAnn bottom s)
+                    (setAnn_annotation bottom s)
+             }.
+Proof.
+  - intros s' s [a Ann].
+    exists (fst (backward (f s') nil nil s a)).
+    eapply backward_annotation; eauto.
+  - intros ? [d Ann]; simpl.
+    pose proof (@ann_bottom s (option (Dom s)) _ _ _ Ann).
+    eapply H0.
+  - intros. eapply terminating_sig.
+    eapply terminating_ann. eapply terminating_option. eauto.
+  - intros s s' [a Ann] [b Bnn] LE; simpl in *.
+    eapply (backward_monotone (f s) (fMon s)); eauto.
 Qed.
 
 (*
