Infra/OptionR.v
@@ -1,0 +1,70 @@
+Require Import Util DecSolve Coq.Classes.RelationClasses Libs.PartialOrder Terminating.
+
+Set Implicit Arguments.
+
+Inductive option_R A B (R: A -> B -> Prop) : option A -> option B -> Prop :=
+| option_R_None : option_R R None None
+| option_R_Some a b : R a b -> option_R R (Some a) (Some b).
+
+Instance option_R_refl A R `{Reflexive A R} : Reflexive (option_R R).
+Proof.
+  unfold Reflexive in *; intros []; eauto using option_R.
+Qed.
+
+Instance option_R_sym A R `{Symmetric A R} : Symmetric (option_R R).
+Proof.
+  unfold Symmetric in *; intros; inv H0; eauto using option_R.
+Qed.
+
+Instance option_R_trans A R `{Transitive A R} : Transitive (option_R R).
+Proof.
+  hnf; intros ? ? ? B C.
+  inv B; inv C; econstructor; eauto.
+Qed.
+
+Instance option_R_equivalence A R `{Equivalence A R} : Equivalence (option_R R).
+Proof.
+  econstructor; eauto with typeclass_instances.
+Qed.
+
+Instance option_R_anti A R Eq `{EqA:Equivalence _ Eq} `{@Antisymmetric A Eq EqA R}
+  : @Antisymmetric _ (option_R Eq) (option_R_equivalence _ _) (option_R R).
+
+Proof.
+  intros ? ? B C. inv B; inv C; eauto using option_R.
+Qed.
+
+Instance option_R_dec A B (R:A->B->Prop)
+         `{forall a b, Computable (R a b)} (a:option A) (b:option B) :
+  Computable (option_R R a b).
+Proof.
+  destruct a,b; try dec_solve.
+  decide (R a b); dec_solve.
+Defined.
+
+Instance PartialOrder_option Dom `{PartialOrder Dom}
+: PartialOrder (option Dom) := {
+  poLe := option_R poLe;
+  poLe_dec := @option_R_dec _ _ poLe poLe_dec;
+  poEq := option_R poEq;
+  poEq_dec := @option_R_dec _ _ poEq poEq_dec;
+}.
+Proof.
+  - intros; inv H0; eauto using option_R, poLe_refl.
+Defined.
+
+
+Instance terminating_option Dom `{PO:PartialOrder Dom}
+  : Terminating Dom poLt
+    -> Terminating (option Dom) poLt.
+Proof.
+  intros. hnf; intros.
+  destruct x.
+  - specialize (H d).
+    general induction H.
+    econstructor; intros. inv H1; inv H2.
+    eapply H0; eauto using option_R.
+    split; eauto. intro. eapply H3; econstructor; eauto.
+  - econstructor; intros. inv H0.
+    exfalso. inv H1. eapply H2; reflexivity.
+Qed.
